Hnr.thy
@@ -1,0 +1,146 @@
+theory Hnr 
+  imports Array_Safe Diff_Arr
+begin
+
+definition hnr where "hnr \<Gamma> c \<Gamma>' R a = <\<Gamma>> c <\<lambda>r. \<Gamma>' * R a r>\<^sub>t"
+
+lemmas hnrD = hnr_def[THEN iffD1]
+lemmas hnrI = hnr_def[THEN iffD2]
+
+definition id_assn where "id_assn a c = \<up>(c = a)"
+
+abbreviation array_assn where "array_assn xs xsi \<equiv> xsi \<mapsto>\<^sub>a xs"
+
+lemma hnr_return: "hnr \<Gamma> (return x) \<Gamma> id_assn x"
+  unfolding hnr_def id_assn_def
+  by sep_auto
+
+lemma hnr_let:
+  assumes 
+    "hnr \<Gamma> vi \<Gamma>\<^sub>1 R\<^sub>1 v" 
+    "\<And>xi x. hnr (\<Gamma>\<^sub>1 * R\<^sub>1 x xi) (fi xi) \<Gamma>' R (f x)"
+  shows 
+    "hnr \<Gamma> (do { x \<leftarrow> vi; fi x }) \<Gamma>' R (let x = v in f x)"
+  supply[sep_heap_rules] = assms[THEN hnrD]
+  apply(rule hnrI)
+  by sep_auto
+
+lemma hnr_if: 
+  assumes
+    "hnr \<Gamma> ai \<Gamma>\<^sub>a R\<^sub>a a"
+    "hnr \<Gamma> bi \<Gamma>\<^sub>b R\<^sub>b b"
+  shows 
+    "hnr 
+      \<Gamma> 
+      (if c then ai else bi) 
+      (\<Gamma>\<^sub>a \<or>\<^sub>A \<Gamma>\<^sub>b) 
+      (\<lambda>a r. R\<^sub>a a r * \<up> c \<or>\<^sub>A R\<^sub>b a r * \<up>(\<not>c)) 
+      (if c then a else b)" 
+  supply[sep_heap_rules] = assms[THEN hnrD]
+  apply(rule hnrI)
+  by(sep_auto simp: ent_star_mono)
+
+(* TODO: 
+lemma hnr_tuple: 
+assumes
+  "hnr \<Gamma> ai \<Gamma>\<^sub>a R\<^sub>a a"
+  "hnr \<Gamma> bi \<Gamma>\<^sub>b R\<^sub>b b"
+shows 
+  "hnr 
+    \<Gamma> 
+    (do { a \<leftarrow> ai; b \<leftarrow> bi; return (a, b) })
+    (\<Gamma>\<^sub>a \<and>\<^sub>A \<Gamma>\<^sub>b) 
+    (\<lambda>(a1, a2) (r1, r2). R\<^sub>a a1 r1 \<and>\<^sub>A R\<^sub>b a2 r2) 
+    (a, b)" 
+  supply[sep_heap_rules] = assms[THEN hnrD]
+  apply(rule hnrI)
+  apply sep_auto
+  apply(rule fi_rule[of "\<Gamma>"])
+  sorry *)
+
+
+lemma hnr_array_nth: "
+    hnr
+     (xsi \<mapsto>\<^sub>a xs * id_assn i ii)
+     (array_nth_safe xsi ii) 
+     (xsi \<mapsto>\<^sub>a xs * id_assn i ii) 
+     id_assn 
+     (xs ! i)"
+  unfolding id_assn_def
+  apply(rule hnrI)
+  by sep_auto
+
+lemma hnr_array_update: "
+    hnr 
+      (xsi \<mapsto>\<^sub>a xs * id_assn i ii * id_assn v vi) 
+      (array_update_safe ii vi xsi) 
+      (id_assn i ii * id_assn v vi) 
+      array_assn 
+      (xs [i:= v])"
+  unfolding id_assn_def
+  apply(rule hnrI)
+  by sep_auto
+
+lemma hnr_pass: "hnr (id_assn x xi) (return xi) emp id_assn x"
+  unfolding id_assn_def
+  apply(rule hnrI)
+  by sep_auto
+
+(* TODO : *)
+lemma hnr_frame:
+  assumes
+    "hnr \<Gamma> fi \<Gamma>' R f"
+    "\<Gamma>\<^sub>P \<Longrightarrow>\<^sub>A \<Gamma> * F"
+  shows
+    "hnr \<Gamma>\<^sub>P fi (\<Gamma>' * F) R f"
+  apply(rule hnrI)
+  by (smt (verit) assms(1) assms(2) assn_aci(10) fi_rule hnrD hoare_triple_def)
+
+lemma hnr_lookup: "
+  hnr
+    (master_assn t * id_assn i ii * \<up>(t \<turnstile> xs \<sim> xsi \<and> i < length xs))
+    (lookup xsi ii)
+    (master_assn t * id_assn i ii * \<up>(t \<turnstile> xs \<sim> xsi \<and> i < length xs))
+    id_assn
+    (xs ! i)"
+  unfolding id_assn_def
+  apply(rule hnrI)
+  using lookup by fastforce
+
+lemma hnr_realize: "
+  hnr
+    (master_assn t * \<up>(t \<turnstile> xs \<sim> xsi))
+    (realize xsi)
+    (master_assn t * \<up>(t \<turnstile> xs \<sim> xsi))
+    array_assn
+    xs"
+  unfolding id_assn_def
+  apply(rule hnrI)
+  using realize[of t xs xsi]
+  by(sep_auto simp: cons_post_rule ent_refl_true)
+
+lemma hnr_update: "
+  hnr
+    (master_assn t * \<up>(t \<turnstile> xs \<sim> xsi \<and> i < length xs) * id_assn i ii * id_assn v vi)
+    (update xsi ii vi)
+    (id_assn i ii * id_assn v vi)
+    (\<lambda>xs xsi. \<exists>\<^sub>At'. master_assn t' * \<up>(t' \<turnstile> xs \<sim> xsi))
+    (xs [i:= v])"
+  unfolding id_assn_def
+  apply(rule hnrI)
+  using update[of t xs xsi i v]
+  by sep_auto
+
+lemma hnr_update': "
+  hnr
+    (master_assn t * \<up>(t \<turnstile> xs \<sim> xsi \<and> i < length xs) * id_assn i ii * id_assn v vi)
+    (update xsi ii vi)
+    (id_assn i ii * id_assn v vi)
+    (\<lambda>_ _. \<exists>\<^sub>At'. master_assn t' * \<up>(\<forall>xs' xsi'. t \<turnstile> xs' \<sim>  xsi' \<longrightarrow> t' \<turnstile> xs' \<sim>  xsi'))
+    (xs [i:= v])"
+  unfolding id_assn_def
+  apply(rule hnrI)
+  using update'[of t xs xsi i v]
+  by sep_auto
+
+end
