Test.thy
@@ -22,12 +22,13 @@ ML_val \<open>@{code test} ()\<close>
 
 export_code test in SML_imp module_name foo
 
-(* HNR *)
+(* Hnr *)
 
 value "(xs[1 := 2], xs[1 := 3])"
 
 definition test1 where
-  "test1 xs = (let c1 = 1; c2 = 2; c3 = 3; t1 = xs[c1 := c2]; t2 = t1[c1 := c3]; t3 = t2 ! c2 in t3)"
+  "test1 xs = 
+    (let c1 = 1; c2 = 2; c3 = 3; t1 = xs[c1 := c2]; t2 = t1[c1 := c3]; t3 = t2 ! c2 in t3)"
 
 schematic_goal "hnr (array_assn xs xsi) (?c :: ?'a Heap) ?\<Gamma>' ?R (test1 xs)"
   unfolding test1_def 
@@ -40,9 +41,6 @@ schematic_goal "hnr (array_assn xs xsi) (?c :: ?'a Heap) ?\<Gamma>' ?R (test1 xs
   apply(rule hnr_frame[OF hnr_pass])
   sorry
   
-
-datatype 'a list = Nil | Cons 'a "'a list"
-
 export_code array_nth_safe array_update_safe in SML_imp
 
 end
